# python_exercises

题:
2   2   2 = 6
3   3   3 = 6
4   4   4 = 6
5   5   5 = 6
6   6   6 = 6
7   7   7 = 6
8   8   8 = 6
9   9   9 = 6
解:

------
2 +  2 +  2 = 6
2 +  2 *  2 = 6
2 *  2 +  2 = 6
------
3 *  3 -  3 = 6
------
√ 4 + √ 4 + √ 4 = 6.0
4 +  4 - √ 4 = 6.0
√ 4 + √ 4 * √ 4 = 6.0
4 +  4 / √ 4 = 6.0
4 - √ 4 +  4 = 6.0
√ 4 * √ 4 + √ 4 = 6.0
4 * √ 4 - √ 4 = 6.0
√ 4 *  4 - √ 4 = 6.0
4 / √ 4 +  4 = 6.0
------
5 +  5 /  5 = 6
5 + √ 5 / √ 5 = 6.0
5 + 3√ 5 / 3√ 5 = 6.0
5 /  5 +  5 = 6
√ 5 / √ 5 +  5 = 6.0
3√ 5 / 3√ 5 +  5 = 6.0
------
6 +  6 -  6 = 6
6 + 3√ 6 - 3√ 6 = 6.0
3√ 6 +  6 - 3√ 6 = 6.0
6 -  6 +  6 = 6
6 - √ 6 + √ 6 = 6.0
6 - 3√ 6 + 3√ 6 = 6.0
√ 6 - √ 6 +  6 = 6.0
3√ 6 - 3√ 6 +  6 = 6.0
6 *  6 /  6 = 6
6 * √ 6 / √ 6 = 6.0
6 * 3√ 6 / 3√ 6 = 6.0
√ 6 *  6 / √ 6 = 6.0
3√ 6 *  6 / 3√ 6 = 6.0
6 /  6 *  6 = 6
6 / √ 6 * √ 6 = 6.0
6 / 3√ 6 * 3√ 6 = 6.0
√ 6 / √ 6 *  6 = 6.0
3√ 6 / 3√ 6 *  6 = 6.0
------
7 -  7 /  7 = 6
7 - √ 7 / √ 7 = 6.0
7 - 3√ 7 / 3√ 7 = 6.0
------
3√ 8 + 3√ 8 + 3√ 8 = 6.0
3√ 8 + 3√ 8 * 3√ 8 = 6.0
3√ 8 +  8 / 3√ 8 = 6.0
3√ 8 * 3√ 8 + 3√ 8 = 6.0
8 / 3√ 8 + 3√ 8 = 6.0
------
√ 9 +  9 / √ 9 = 6.0
9 -  9 / √ 9 = 6.0
√ 9 * √ 9 - √ 9 = 6.0
9 / √ 9 + √ 9 = 6.0
